Extract split specification from set theories

BPlusTree_ImpSet.thy
@@ -1,7 +1,7 @@
 theory BPlusTree_ImpSet
   imports
-    BPlusTree_Imp
     BPlusTree_Set
+    BPlusTree_ImpSplitSpec
     "HOL-Real_Asymp.Inst_Existentials"
 begin
 
@@ -9,100 +9,6 @@ section "Imperative Set operations"
 
 subsection "Auxiliary operations"
 
-definition "split_relation xs \<equiv>
-   \<lambda>(as,bs) i. i \<le> length xs \<and> as = take i xs \<and> bs = drop i xs"
-
-lemma split_relation_alt: 
-  "split_relation as (ls,rs) i = (as = ls@rs \<and> i = length ls)"
-  by (auto simp add: split_relation_def)
-
-
-lemma split_relation_length: "split_relation xs (ls,rs) (length xs) = (ls = xs \<and> rs = [])"
-  by (simp add: split_relation_def)
-
-(* auxiliary lemmas on assns *)
-(* simp? not sure if it always makes things more easy *)
-lemma list_assn_prod_map: "list_assn (A \<times>\<^sub>a B) xs ys = list_assn B (map snd xs) (map snd ys) * list_assn A (map fst xs) (map fst ys)"
-  apply(induct "(A \<times>\<^sub>a B)" xs ys rule: list_assn.induct)
-     apply(auto simp add: ab_semigroup_mult_class.mult.left_commute ent_star_mono star_aci(2) star_assoc)
-  done
-
-(* concrete *)
-lemma id_assn_list: "h \<Turnstile> list_assn id_assn (xs::'a list) ys \<Longrightarrow> xs = ys"
-  apply(induction "id_assn::('a \<Rightarrow> 'a \<Rightarrow> assn)" xs ys rule: list_assn.induct)
-     apply(auto simp add: less_Suc_eq_0_disj pure_def)
-  done
-
-lemma id_assn_list_alt: "list_assn id_assn (xs::'a list) ys = \<up>(xs = ys)"
-  apply(induction "id_assn::('a \<Rightarrow> 'a \<Rightarrow> assn)" xs ys rule: list_assn.induct)
-     apply(auto simp add: less_Suc_eq_0_disj pure_def)
-  done
-
-
-lemma snd_map_help:
-  "x \<le> length tsi \<Longrightarrow>
-       (\<forall>j<x. snd (tsi ! j) = ((map snd tsi)!j))"
-  "x < length tsi \<Longrightarrow> snd (tsi!x) = ((map snd tsi)!x)"
-  by auto
-
-
-lemma split_ismeq: "((a::nat) \<le> b \<and> X) = ((a < b \<and> X) \<or> (a = b \<and> X))"
-  by auto
-
-lemma split_relation_map: "split_relation as (ls,rs) i \<Longrightarrow> split_relation (map f as) (map f ls, map f rs) i"
-  apply(induction as arbitrary: ls rs i)
-   apply(auto simp add: split_relation_def take_map drop_Cons')
-  apply(metis list.simps(9) take_map)
-  done
-
-lemma split_relation_access: "\<lbrakk>split_relation as (ls,rs) i; rs = r#rrs\<rbrakk> \<Longrightarrow> as!i = r"
-  by (simp add: split_relation_alt)
-
-
-
-lemma index_to_elem_all: "(\<forall>j<length xs. P (xs!j)) = (\<forall>x \<in> set xs. P x)"
-  by (simp add: all_set_conv_nth)
-
-lemma index_to_elem: "n < length xs \<Longrightarrow> (\<forall>j<n. P (xs!j)) = (\<forall>x \<in> set (take n xs). P x)"
-  by (simp add: all_set_conv_nth)
-    (* ----------------- *)
-
-definition split_half :: "'a::heap pfarray \<Rightarrow> nat Heap"
-  where
-    "split_half a \<equiv> do {
-  l \<leftarrow> pfa_length a;
-  return ((l + 1) div 2)
-}"
-
-lemma split_half_rule[sep_heap_rules]: "<
-    is_pfa c tsi a>
-    split_half a
-  <\<lambda>i. 
-      is_pfa c tsi a
-    * \<up>(i = (length tsi + 1) div 2 \<and>  split_relation tsi (BPlusTree_Set.split_half tsi) i)>"
-  unfolding split_half_def split_relation_def
-  apply(rule hoare_triple_preI)
-  apply(sep_auto dest!: list_assn_len mod_starD)
-  done
-
-
-subsection "The imperative split locale"
-
-locale imp_split_tree = abs_split_tree: BPlusTree_Set.split_tree split
-  for split::
-    "('a::{heap,default,linorder,order_top} bplustree \<times> 'a) list \<Rightarrow> 'a
-       \<Rightarrow> ('a bplustree \<times> 'a) list \<times> ('a bplustree \<times> 'a) list" +
-  fixes imp_split:: "('a btnode ref option \<times> 'a::{heap,default,linorder,order_top}) pfarray \<Rightarrow> 'a \<Rightarrow> nat Heap"
-  assumes imp_split_rule [sep_heap_rules]:"sorted_less (separators ts) \<Longrightarrow>
-  length tsi = length rs \<Longrightarrow>
-  tsi'' = zip (zip (map fst tsi) (zip (butlast (r#rs)) (butlast (rs@[z])))) (map snd tsi) \<Longrightarrow>
- <is_pfa c tsi (a,n) 
-  * blist_assn k ts tsi'' > 
-    imp_split (a,n) p 
-  <\<lambda>i. 
-    is_pfa c tsi (a,n)
-    * blist_assn k ts tsi''
-    * \<up>(split_relation ts (split ts p) i)>\<^sub>t"
 
 text "This locale extends the abstract split locale,
 assuming that we are provided with an imperative program
@@ -453,7 +359,7 @@ proof -
     done
 qed
 
-lemma "BPlusTree_Set.split_half ts = (ls,rs) \<Longrightarrow> length ls = Suc (length ts) div 2"
+lemma "BPlusTree_SplitSpec.split_half ts = (ls,rs) \<Longrightarrow> length ls = Suc (length ts) div 2"
   by (metis Suc_eq_plus1 split_half_conc)
 
 
@@ -483,7 +389,7 @@ proof (cases "length ts \<le> 2*k")
 next
   case [simp]: False
   then obtain ls sub sep rs where      
-    split_half_eq: "BPlusTree_Set.split_half ts = (ls@[(sub,sep)],rs)"
+    split_half_eq: "BPlusTree_SplitSpec.split_half ts = (ls@[(sub,sep)],rs)"
     using abs_split.node\<^sub>i_cases by blast
   then show ?thesis
     apply(subst node\<^sub>i_def)
@@ -704,7 +610,7 @@ proof (cases "length xs \<le> 2*k")
 next
   case [simp]: False
   then obtain ls sep rs where
-    split_half_eq: "BPlusTree_Set.split_half xs = (ls@[sep],rs)"
+    split_half_eq: "BPlusTree_SplitSpec.split_half xs = (ls@[sep],rs)"
     using abs_split.Lnode\<^sub>i_cases by blast
   then show ?thesis
     apply(subst Lnode\<^sub>i_def)
@@ -1502,7 +1408,7 @@ lemma btupi_assn_T: "h \<Turnstile> btupi_assn k (abs_split.node\<^sub>i k ts t)
 
 lemma btupi_assn_Up: "h \<Turnstile> btupi_assn k (abs_split.node\<^sub>i k ts t) (Up\<^sub>i l a r) r' z \<Longrightarrow>
   abs_split.node\<^sub>i k ts t = (
-    case BPlusTree_Set.split_half ts of (ls,rs) \<Rightarrow> (
+    case BPlusTree_SplitSpec.split_half ts of (ls,rs) \<Rightarrow> (
       case last ls of (sub,sep) \<Rightarrow>
         abs_split.Up\<^sub>i (Node (butlast ls) sub) sep (Node rs t)
   )
@@ -1517,7 +1423,7 @@ lemma Lbtupi_assn_T: "h \<Turnstile> btupi_assn k (abs_split.Lnode\<^sub>i k ts)
 
 lemma Lbtupi_assn_Up: "h \<Turnstile> btupi_assn k (abs_split.Lnode\<^sub>i k ts) (Up\<^sub>i l a r) r' z \<Longrightarrow>
   abs_split.Lnode\<^sub>i k ts = (
-    case BPlusTree_Set.split_half ts of (ls,rs) \<Rightarrow> (
+    case BPlusTree_SplitSpec.split_half ts of (ls,rs) \<Rightarrow> (
       case last ls of sep \<Rightarrow>
         abs_split.Up\<^sub>i (LNode ls) sep (LNode rs)
   )
@@ -2271,7 +2177,7 @@ lemma delete_rule:
 
 end
 
-locale imp_split_list = abs_split_list: BPlusTree_Set.split_list split_list
+locale imp_split_list = abs_split_list: BPlusTree_SplitSpec.split_list split_list
   for split_list::
     "('a::{heap,default,linorder,order_top}) list \<Rightarrow> 'a
        \<Rightarrow> 'a list \<times> 'a list" +
