BPlusTree_Set.thy
@@ -1,33 +1,11 @@
 theory BPlusTree_Set
-  imports BPlusTree
+  imports
+    BPlusTree_SplitSpec
     "HOL-Data_Structures.Set_Specs"
 begin
 
 
 section "Set interpretation"
-
-subsection "Auxiliary functions"
-
-(* a version of split half that assures the left side to be non-empty *)
-fun split_half:: "_ list \<Rightarrow> _ list \<times> _ list" where
-  "split_half xs = (take ((length xs + 1) div 2) xs, drop ((length xs + 1) div 2) xs)"
-
-lemma split_half_conc: "split_half xs = (ls, rs) = (xs = ls@rs \<and> length ls = (length xs + 1) div 2)"
-  by force
-
-lemma drop_not_empty: "xs \<noteq> [] \<Longrightarrow> drop (length xs div 2) xs \<noteq> []"
-  apply(induction xs)
-   apply(auto split!: list.splits)
-  done
-
-lemma take_not_empty: "xs \<noteq> [] \<Longrightarrow> take ((length xs + 1) div 2) xs \<noteq> []"
-  apply(induction xs)
-   apply(auto split!: list.splits)
-  done
-
-lemma split_half_not_empty: "length xs \<ge> 1 \<Longrightarrow> \<exists>ls a rs. split_half xs = (ls@[a],rs)"
-  using take_not_empty
-  by (metis (no_types, hide_lams) Ex_list_of_length One_nat_def le_trans length_Cons list.size(4) nat_1_add_1 not_one_le_zero rev_exhaust split_half.simps take0 take_all_iff)
 
 (* obsolete fact *)
 lemma insert_list_length[simp]:
@@ -80,26 +58,6 @@ lemma del_list_length[simp]:
   using delete_list_length[of ks ins_list k]
   by (simp add: assms set_del_list sorted_del_list)
 
-subsection "The split function locale"
-
-text "Here, we abstract away the inner workings of the split function
-      for B-tree operations."
-
-locale split_tree =
-  fixes split ::  "('a bplustree\<times>'a::{linorder,order_top}) list \<Rightarrow> 'a \<Rightarrow> (('a bplustree\<times>'a) list \<times> ('a bplustree\<times>'a) list)"
-  assumes split_req:
-    "\<lbrakk>split xs p = (ls,rs)\<rbrakk> \<Longrightarrow> xs = ls @ rs"
-    "\<lbrakk>split xs p = (ls@[(sub,sep)],rs); sorted_less (separators xs)\<rbrakk> \<Longrightarrow> sep < p"
-    "\<lbrakk>split xs p = (ls,(sub,sep)#rs); sorted_less (separators xs)\<rbrakk> \<Longrightarrow> p \<le> sep"
-begin
-  lemmas split_conc = split_req(1)
-  lemmas split_sorted = split_req(2,3)
-  
-  
-  lemma [termination_simp]:"(ls, (sub, sep) # rs) = split ts y \<Longrightarrow>
-        size sub < Suc (size_list (\<lambda>x. Suc (size (fst x))) ts  + size l)"
-    using split_conc[of ts y ls "(sub,sep)#rs"] by auto
-end
 
 (* TODO what if we define a function "list_split" that returns
  a split list for mapping arbitrary f (separators) and g (subtrees)
