BPlusTree_ImpSplitSpec.thy
@@ -1,0 +1,100 @@
+theory BPlusTree_ImpSplitSpec
+imports BPlusTree_Imp BPlusTree_SplitSpec
+begin
+
+definition "split_relation xs \<equiv>
+   \<lambda>(as,bs) i. i \<le> length xs \<and> as = take i xs \<and> bs = drop i xs"
+
+lemma split_relation_alt: 
+  "split_relation as (ls,rs) i = (as = ls@rs \<and> i = length ls)"
+  by (auto simp add: split_relation_def)
+
+
+lemma split_relation_length: "split_relation xs (ls,rs) (length xs) = (ls = xs \<and> rs = [])"
+  by (simp add: split_relation_def)
+
+(* auxiliary lemmas on assns *)
+(* simp? not sure if it always makes things more easy *)
+lemma list_assn_prod_map: "list_assn (A \<times>\<^sub>a B) xs ys = list_assn B (map snd xs) (map snd ys) * list_assn A (map fst xs) (map fst ys)"
+  apply(induct "(A \<times>\<^sub>a B)" xs ys rule: list_assn.induct)
+     apply(auto simp add: ab_semigroup_mult_class.mult.left_commute ent_star_mono star_aci(2) star_assoc)
+  done
+
+(* concrete *)
+lemma id_assn_list: "h \<Turnstile> list_assn id_assn (xs::'a list) ys \<Longrightarrow> xs = ys"
+  apply(induction "id_assn::('a \<Rightarrow> 'a \<Rightarrow> assn)" xs ys rule: list_assn.induct)
+     apply(auto simp add: less_Suc_eq_0_disj pure_def)
+  done
+
+lemma id_assn_list_alt: "list_assn id_assn (xs::'a list) ys = \<up>(xs = ys)"
+  apply(induction "id_assn::('a \<Rightarrow> 'a \<Rightarrow> assn)" xs ys rule: list_assn.induct)
+     apply(auto simp add: less_Suc_eq_0_disj pure_def)
+  done
+
+
+lemma snd_map_help:
+  "x \<le> length tsi \<Longrightarrow>
+       (\<forall>j<x. snd (tsi ! j) = ((map snd tsi)!j))"
+  "x < length tsi \<Longrightarrow> snd (tsi!x) = ((map snd tsi)!x)"
+  by auto
+
+
+lemma split_ismeq: "((a::nat) \<le> b \<and> X) = ((a < b \<and> X) \<or> (a = b \<and> X))"
+  by auto
+
+lemma split_relation_map: "split_relation as (ls,rs) i \<Longrightarrow> split_relation (map f as) (map f ls, map f rs) i"
+  apply(induction as arbitrary: ls rs i)
+   apply(auto simp add: split_relation_def take_map drop_Cons')
+  apply(metis list.simps(9) take_map)
+  done
+
+lemma split_relation_access: "\<lbrakk>split_relation as (ls,rs) i; rs = r#rrs\<rbrakk> \<Longrightarrow> as!i = r"
+  by (simp add: split_relation_alt)
+
+
+
+lemma index_to_elem_all: "(\<forall>j<length xs. P (xs!j)) = (\<forall>x \<in> set xs. P x)"
+  by (simp add: all_set_conv_nth)
+
+lemma index_to_elem: "n < length xs \<Longrightarrow> (\<forall>j<n. P (xs!j)) = (\<forall>x \<in> set (take n xs). P x)"
+  by (simp add: all_set_conv_nth)
+    (* ----------------- *)
+
+definition split_half :: "'a::heap pfarray \<Rightarrow> nat Heap"
+  where
+    "split_half a \<equiv> do {
+  l \<leftarrow> pfa_length a;
+  return ((l + 1) div 2)
+}"
+
+lemma split_half_rule[sep_heap_rules]: "<
+    is_pfa c tsi a>
+    split_half a
+  <\<lambda>i. 
+      is_pfa c tsi a
+    * \<up>(i = (length tsi + 1) div 2 \<and>  split_relation tsi (BPlusTree_SplitSpec.split_half tsi) i)>"
+  unfolding split_half_def split_relation_def
+  apply(rule hoare_triple_preI)
+  apply(sep_auto dest!: list_assn_len mod_starD)
+  done
+
+
+subsection "The imperative split locale"
+
+locale imp_split_tree = abs_split_tree: BPlusTree_SplitSpec.split_tree split
+  for split::
+    "('a::{heap,default,linorder,order_top} bplustree \<times> 'a) list \<Rightarrow> 'a
+       \<Rightarrow> ('a bplustree \<times> 'a) list \<times> ('a bplustree \<times> 'a) list" +
+  fixes imp_split:: "('a btnode ref option \<times> 'a::{heap,default,linorder,order_top}) pfarray \<Rightarrow> 'a \<Rightarrow> nat Heap"
+  assumes imp_split_rule [sep_heap_rules]:"sorted_less (separators ts) \<Longrightarrow>
+  length tsi = length rs \<Longrightarrow>
+  tsi'' = zip (zip (map fst tsi) (zip (butlast (r#rs)) (butlast (rs@[z])))) (map snd tsi) \<Longrightarrow>
+ <is_pfa c tsi (a,n) 
+  * blist_assn k ts tsi'' > 
+    imp_split (a,n) p 
+  <\<lambda>i. 
+    is_pfa c tsi (a,n)
+    * blist_assn k ts tsi''
+    * \<up>(split_relation ts (split ts p) i)>\<^sub>t"
+
+end
